src/Narcissus/Examples/IPTables.v
@@ -189,15 +189,16 @@ Notation "cf '-j' result" :=
   (rule_from_condition cf.(cf_cond) result)
     (at level 41, left associativity).
 
-Notation "n , m" :=
+Notation "n ' m" :=
   ((n * (N.of_nat 256) + m)%N)
-    (at level 38, format "n , m", left associativity)
+    (at level 38, format "n ' m", left associativity)
   : addr_scope.
+Bind Scope addr_scope with N.
 
 Notation "cf !" :=
   {| cf_cond := cf.(cf_cond);
      cf_negate_next := negb cf.(cf_negate_next) |}
-    (at level 42, left associativity).
+    (at level 43, left associativity).
 
 Definition iptables :=
   {| cf_cond := fun i: input => true;
@@ -209,22 +210,22 @@ Require Import IPTablesPorts.
 
 Example drop_messages_192_10 :=
   iptables -A FORWARD
-           --source 192,0,0,0/8
-           --destination 10,0,0,0/8
+           --source 192'0'0'0/8
+           --destination 10'0'0'0/8
            -j DROP.
 
 Example drop_dhcp_serverport_from_nonserver :=
   iptables -A FORWARD
            --protocol "UDP"
            --source-port bootps
-           ! --source 192,168,0,1
+           ! --source 192'168'0'1
            -j DROP.
 
 Example accept_dhcp_client_broadcast :=
   iptables -A FORWARD
            --protocol "UDP"
            --source-port bootpc
-           --destination 255,255,255,255
+           --destination 255'255'255'255
            -j ACCEPT.
 
 Example drop_dhcp_messages_to_wrong_port :=
@@ -238,7 +239,7 @@ Example drop_dhcp_messages_to_wrong_address :=
   iptables -A FORWARD
            --protocol "UDP"
            --source-port bootpc
-           ! --destination 255,255,255,255/32
+           ! --destination 255'255'255'255/32
            -j DROP.
 
 (** We can apply these filters to packets: *)
@@ -357,5 +358,5 @@ Eval cbv zeta in
     ltac:(simp (iptables -A FORWARD
                          --protocol "UDP"
                          --source-port bootpc
-                         --destination 255255,255,255
+                         --destination 255'255'255'255
                          -j ACCEPT)).
